Add formalization of constraint reduction

Deduction.thy
@@ -57,4 +57,66 @@ shows "H \<turnstile> u"
   by(induction "insert t H" u rule:deduce.induct) (auto intro:deduce.intros)
 
 
+datatype constraint =
+Constraint "msg list" "msg list" "msg" ( "((2_/|_)/ \<Zrres>_) " [67,67,67]66)
+
+type_synonym constraint_system = "constraint list"
+
+fun fv_constraint::"constraint \<Rightarrow> string set" where
+"fv_constraint (M | A  \<Zrres> t) = \<Union>(set(map fv_msg M)) \<union>  \<Union>(set(map fv_msg A)) \<union> fv_msg t"
+
+fun fv_constraint_system::"constraint_system \<Rightarrow> string set" where
+"fv_constraint_system cs = \<Union>(set(map fv_constraint cs))"
+
+fun sapply_constraint::"subst_msg \<Rightarrow> constraint \<Rightarrow> constraint" where
+"sapply_constraint \<sigma> (M | A \<Zrres> t) = map (sapply_msg \<sigma>) M | map  (sapply_msg \<sigma>) A \<Zrres>  sapply_msg \<sigma> t"
+
+fun sapply_constraint_system::"subst_msg \<Rightarrow> constraint_system \<Rightarrow> constraint_system" where
+"sapply_constraint_system \<sigma> cs = map (sapply_constraint \<sigma>) cs"
+
+(*add main lemmas(?) about fv and sapply*)
+
+definition sol::"constraint_system \<Rightarrow> subst_msg set" where
+"sol cs = {\<sigma> | M A t \<sigma>. (M | A \<Zrres> t) \<in> set(cs) \<longrightarrow> set(map (sapply_msg \<sigma>) (M@A)) \<turnstile> sapply_msg \<sigma> t}"
+
+lemma "sol (cs1@cs2 ) = sol (cs1 ) \<inter> sol (cs2)"
+  sorry
+
+lemma "\<tau> \<in> sol (sapply_constraint_system \<sigma> cs) \<Longrightarrow> scomp_msg \<tau> \<sigma> \<in> sol cs"
+  sorry
+
+fun is_variable::"msg \<Rightarrow> bool" where
+"is_variable (Variable _) = True"
+| "is_variable _ = False"
+
+inductive rer1 :: "constraint \<Rightarrow> subst_msg \<Rightarrow> constraint_system \<Rightarrow> bool"
+("(_)/\<leadsto>\<^sub>1[_]/ (_)" [64,64,64]63) where
+Unifl: "\<lbrakk>\<not> is_variable t; u \<in> set(M) \<union> set(A); sapply_msg \<sigma> u = sapply_msg \<sigma> t\<rbrakk> 
+          \<Longrightarrow> M | A \<Zrres> t \<leadsto>\<^sub>1[\<sigma>] Nil"
+
+| CompHashl: "M | A \<Zrres> (\<h> t) \<leadsto>\<^sub>1[Variable] [M | A \<Zrres> t]"
+| CompPairl: "M | A \<Zrres> (\<langle>t1,t2\<rangle>) \<leadsto>\<^sub>1[Variable] [M | A \<Zrres> t1, M | A \<Zrres> t2]"
+| CompSencl: "M | A \<Zrres> (\<lbrace>t\<rbrace>\<^sub>k) \<leadsto>\<^sub>1[Variable] [M | A \<Zrres> t, M | A \<Zrres> k]"
+| CompAencl: "M | A \<Zrres> ({t}\<^sub>k) \<leadsto>\<^sub>1[Variable] [M | A \<Zrres> t, M | A \<Zrres> k]"
+| CompSignl: "M | A \<Zrres> ([t]\<^sub>\<iota>) \<leadsto>\<^sub>1[Variable] [M | A \<Zrres> t]"
+
+| Projl: "((\<langle>u,v\<rangle>)#M) | A \<Zrres> t \<leadsto>\<^sub>1[Variable] [(u#v#M) | ((\<langle>u,v\<rangle>)#A) \<Zrres> t]"
+| Sdecl: "((\<lbrace>u\<rbrace>\<^sub>k)#M) | A \<Zrres> t \<leadsto>\<^sub>1[Variable] [(u#M) | ((\<lbrace>u\<rbrace>\<^sub>k)#A) \<Zrres> t, M | ((\<lbrace>u\<rbrace>\<^sub>k)#A) \<Zrres> k]"
+| Adecl: "(({u}\<^sub>\<iota>)#M) | A \<Zrres> t \<leadsto>\<^sub>1[Variable] [(u#M) | ((\<lbrace>u\<rbrace>\<^sub>\<iota>)#A) \<Zrres> t]"
+| Ksubl:  "(let y = Variable x in (({u}\<^sub>y)#M)) | A \<Zrres> t \<leadsto>\<^sub>1[(Variable(x:=i))] 
+            [sapply_constraint (Variable(x:=i)) ((let y = Variable x in (({u}\<^sub>y)#M)) | A \<Zrres> t)]"
+
+inductive rer :: "constraint_system \<Rightarrow>subst_msg \<Rightarrow> constraint_system \<Rightarrow> bool"
+("_/ \<leadsto>[_]/ _ " [73,73,73]72) where
+Context: "c \<leadsto>\<^sub>1[\<sigma>] cs \<Longrightarrow> (c#cs') \<leadsto>[\<sigma>] (cs@cs')"
+
+inductive rer_star :: "constraint_system \<Rightarrow>subst_msg \<Rightarrow> constraint_system \<Rightarrow> bool"
+("_/ \<leadsto>\<^emph>[_]/ _ " [73,73,73]72) where
+Refl: "cs \<leadsto>\<^emph>[Variable] cs"
+| Trans: "\<lbrakk>cs \<leadsto>[\<sigma>] cs''; cs'' \<leadsto>\<^emph>[\<tau>] cs'\<rbrakk> \<Longrightarrow> cs \<leadsto>\<^emph>[\<tau> \<circ>\<^sub>s \<sigma>] cs'"
+
+
+lemma "[Const ''a''] | [] \<Zrres> Const ''a''  \<leadsto>\<^sub>1[Variable] []"
+  by (auto intro: rer1.intros)
+
 end
